Tap

DeBruijnSSA/BinSyntax/Rewrite.lean
@@ -23,6 +23,8 @@ inductive Region.Beta (Γ : Ctx α ε) : Region φ → Region φ → Prop
     : e.infEffect Γ = ⊥ → Beta Γ (r.let1 e) (r.vsubst e.subst0)
   | let2 (a : Term φ) (b : Term φ) (r : Region φ)
     : a.infEffect Γ = ⊥ → b.infEffect Γ = ⊥ → Beta Γ (r.let2 (a.pair b)) (r.vsubst (a.subst₂ b))
+  | case_left (e : Term φ) (r : Region φ) (s : Region φ) : Beta Γ (case e.inl r s) (let1 e r)
+  | case_right (e : Term φ) (r : Region φ) (s : Region φ) : Beta Γ (case e.inr r s) (let1 e s)
 
 theorem Region.Beta.let1_pure {Γ : Ctx α ε} {e} {r r' : Region φ}
   (h : Region.Beta Γ (r.let1 e) r') : e.infEffect Γ = ⊥ := by cases h; assumption
@@ -39,10 +41,21 @@ theorem Region.Beta.let2_right_pure {Γ : Ctx α ε} {a b : Term φ} {r r' : Reg
 theorem Region.Beta.let2_trg {Γ : Ctx α ε} {a b : Term φ} {r r' : Region φ}
   (h : Region.Beta Γ (r.let2 (a.pair b)) r') : r' = r.vsubst (a.subst₂ b) := by cases h; rfl
 
+theorem Region.Beta.case_left_trg {Γ : Ctx α ε} {e} {r s r' : Region φ}
+  (h : Region.Beta Γ (case e.inl r s) r') : r' = r.let1 e := by cases h; rfl
+
+theorem Region.Beta.case_right_trg {Γ : Ctx α ε} {e} {r s s' : Region φ}
+  (h : Region.Beta Γ (case e.inr r s) s') : s' = s.let1 e := by cases h; rfl
+
 def Region.Beta.WfD {Γ : Ctx α ε} {r r' : Region φ}
   : Region.Beta Γ r r' → r.WfD Γ A → r'.WfD Γ A
   | h, WfD.let1 de dr => h.let1_trg ▸ dr.vsubst (h.let1_pure ▸ de.toInfEffect.subst0)
   | h, WfD.let2 (Term.WfD.pair da db) dr => h.let2_trg ▸
     dr.vsubst ((h.let2_left_pure ▸ da.toInfEffect).subst₂ (h.let2_right_pure ▸ db.toInfEffect))
+  | h, WfD.case (Term.WfD.inl de) dr _ => h.case_left_trg ▸ dr.let1 de
+  | h, WfD.case (Term.WfD.inr de) _ ds => h.case_right_trg ▸ ds.let1 de
+
+-- inductive Region.FuseLet (Γ : Ctx α ε) : Region φ → Region φ → Region φ → Prop
+--   | fuse (e : Term φ) (r : Region φ) (s : Region φ)
 
 end BinSyntax
